Weidenbach_Book/Two_Watched_Literals_Watch_List_Domain.thy
@@ -605,6 +605,82 @@ proof -
   then show ?thesis by (auto simp: uint_max_def)
 qed
 
+lemma twl_struct_invs_is_\<L>\<^sub>a\<^sub>l\<^sub>l_clauses_init_clss:
+  fixes S\<^sub>0 :: \<open>nat twl_st_wl\<close>
+  defines \<open>S \<equiv> twl_st_of_wl None S\<^sub>0\<close>
+  defines \<open>clss \<equiv> (all_lits_of_mm (cdcl\<^sub>W_restart_mset.clauses (state\<^sub>W_of S)))\<close>
+  defines \<open>init \<equiv> (all_lits_of_mm (init_clss (state\<^sub>W_of S)))\<close>
+  assumes invs: \<open>twl_struct_invs (twl_st_of_wl None S\<^sub>0)\<close>
+  shows \<open>is_\<L>\<^sub>a\<^sub>l\<^sub>l clss \<longleftrightarrow> is_\<L>\<^sub>a\<^sub>l\<^sub>l init\<close>
+proof -
+
+  have \<open>cdcl\<^sub>W_restart_mset.no_strange_atm (state\<^sub>W_of S)\<close>
+    using invs unfolding twl_struct_invs_def cdcl\<^sub>W_restart_mset.cdcl\<^sub>W_all_struct_inv_def S_def
+    by fast
+  then have
+    \<open>set_mset clss = set_mset init\<close>
+    unfolding clss_def init_def S_def
+    by (cases S\<^sub>0) (auto simp: clauses_def mset_take_mset_drop_mset' cdcl\<^sub>W_restart_mset_state
+        cdcl\<^sub>W_restart_mset.no_strange_atm_def in_all_lits_of_mm_ain_atms_of_iff)
+  then show \<open>is_\<L>\<^sub>a\<^sub>l\<^sub>l clss \<longleftrightarrow> is_\<L>\<^sub>a\<^sub>l\<^sub>l init\<close>
+    unfolding is_\<L>\<^sub>a\<^sub>l\<^sub>l_def by blast
+qed
+
+lemma literals_are_\<L>\<^sub>i\<^sub>n_conflict_literals_are_in_\<L>\<^sub>i\<^sub>n:
+  assumes
+    \<A>\<^sub>i\<^sub>n: \<open>literals_are_\<L>\<^sub>i\<^sub>n S\<close> and
+    confl: \<open>get_conflict_wl S \<noteq> None\<close> and
+    struct: \<open>twl_struct_invs (twl_st_of_wl None S)\<close>
+  shows \<open>literals_are_in_\<L>\<^sub>i\<^sub>n (the (get_conflict_wl S))\<close>
+proof -
+  have alien: \<open>cdcl\<^sub>W_restart_mset.no_strange_atm (state\<^sub>W_of (twl_st_of_wl None S))\<close>
+    using struct unfolding twl_struct_invs_def cdcl\<^sub>W_restart_mset.cdcl\<^sub>W_all_struct_inv_def
+    by fast
+  then have N: \<open>atms_of (the (get_conflict_wl S)) \<subseteq> atms_of_mm (init_clss (state\<^sub>W_of (twl_st_of_wl None S)))\<close>
+    using confl unfolding cdcl\<^sub>W_restart_mset.no_strange_atm_def
+    by (cases S; cases \<open>get_conflict_wl S\<close>)
+       (auto simp: cdcl\<^sub>W_restart_mset_state mset_take_mset_drop_mset')
+
+  have \<open>is_\<L>\<^sub>a\<^sub>l\<^sub>l (all_lits_of_mm (init_clss (state\<^sub>W_of (twl_st_of_wl None S))))\<close>
+    using twl_struct_invs_is_\<L>\<^sub>a\<^sub>l\<^sub>l_clauses_init_clss[OF struct] \<A>\<^sub>i\<^sub>n by fast
+  then show ?thesis
+    using N in_all_lits_of_m_ain_atms_of_iff in_all_lits_of_mm_ain_atms_of_iff
+    by (fastforce simp: literals_are_in_\<L>\<^sub>i\<^sub>n_def is_\<L>\<^sub>a\<^sub>l\<^sub>l_def )
+qed
+
+lemma set_mset_set_mset_eq_iff: \<open>set_mset A = set_mset B \<longleftrightarrow> (\<forall>a\<in>#A. a \<in># B) \<and> (\<forall>a\<in>#B. a \<in># A)\<close>
+  by blast
+
+lemma is_\<L>\<^sub>a\<^sub>l\<^sub>l_alt_def: \<open>is_\<L>\<^sub>a\<^sub>l\<^sub>l (all_lits_of_mm A) \<longleftrightarrow> atms_of_mm A = atms_of \<L>\<^sub>a\<^sub>l\<^sub>l\<close>
+  unfolding set_mset_set_mset_eq_iff is_\<L>\<^sub>a\<^sub>l\<^sub>l_def Ball_def in_\<L>\<^sub>a\<^sub>l\<^sub>l_atm_of_in_atms_of_iff
+    in_all_lits_of_mm_ain_atms_of_iff
+  by auto (metis literal.sel(2))+
+
+lemma literals_are_\<L>\<^sub>i\<^sub>n_trail_literals_are_in_\<L>\<^sub>i\<^sub>n:
+  assumes
+    \<A>\<^sub>i\<^sub>n: \<open>literals_are_\<L>\<^sub>i\<^sub>n S\<close> and
+    struct: \<open>twl_struct_invs (twl_st_of_wl None S)\<close>
+  shows \<open>literals_are_in_\<L>\<^sub>i\<^sub>n_trail (get_trail_wl S)\<close>
+proof -
+  have alien: \<open>cdcl\<^sub>W_restart_mset.no_strange_atm (state\<^sub>W_of (twl_st_of_wl None S))\<close>
+    using struct unfolding twl_struct_invs_def cdcl\<^sub>W_restart_mset.cdcl\<^sub>W_all_struct_inv_def
+    by fast
+  then have N: \<open>atm_of ` lits_of_l (trail (state\<^sub>W_of (twl_st_of_wl None S)))
+    \<subseteq> atms_of_mm (init_clss (state\<^sub>W_of (twl_st_of_wl None S)))\<close>
+    unfolding cdcl\<^sub>W_restart_mset.no_strange_atm_def
+    by (cases S)
+       (auto simp: cdcl\<^sub>W_restart_mset_state mset_take_mset_drop_mset')
+
+  have \<open>is_\<L>\<^sub>a\<^sub>l\<^sub>l (all_lits_of_mm (init_clss (state\<^sub>W_of (twl_st_of_wl None S))))\<close>
+    using twl_struct_invs_is_\<L>\<^sub>a\<^sub>l\<^sub>l_clauses_init_clss[OF struct] \<A>\<^sub>i\<^sub>n by fast
+  then show ?thesis
+    using N in_all_lits_of_m_ain_atms_of_iff in_all_lits_of_mm_ain_atms_of_iff
+    by (cases S)
+       (auto simp: literals_are_in_\<L>\<^sub>i\<^sub>n_trail_def is_\<L>\<^sub>a\<^sub>l\<^sub>l_alt_def trail.simps
+      lits_of_def image_image init_clss.simps mset_take_mset_drop_mset'
+      atms_of_\<L>\<^sub>a\<^sub>l\<^sub>l_\<A>\<^sub>i\<^sub>n in_\<L>\<^sub>a\<^sub>l\<^sub>l_atm_of_in_atms_of_iff convert_lits_l_def)
+qed
+
 definition (in isasat_input_ops) unit_prop_body_wl_D_inv where
 \<open>unit_prop_body_wl_D_inv T' i L \<longleftrightarrow>
     unit_prop_body_wl_inv T' i L \<and> literals_are_\<L>\<^sub>i\<^sub>n T' \<and> L \<in> snd ` D\<^sub>0
@@ -983,27 +1059,6 @@ definition (in isasat_input_ops) skip_and_resolve_loop_wl_D :: "nat twl_st_wl \<
     }
   \<close>
 
-lemma twl_struct_invs_is_\<L>\<^sub>a\<^sub>l\<^sub>l_clauses_init_clss:
-  fixes S\<^sub>0 :: \<open>nat twl_st_wl\<close>
-  defines \<open>S \<equiv> twl_st_of_wl None S\<^sub>0\<close>
-  defines \<open>clss \<equiv> (all_lits_of_mm (cdcl\<^sub>W_restart_mset.clauses (state\<^sub>W_of S)))\<close>
-  defines \<open>init \<equiv> (all_lits_of_mm (init_clss (state\<^sub>W_of S)))\<close>
-  assumes invs: \<open>twl_struct_invs (twl_st_of_wl None S\<^sub>0)\<close>
-  shows \<open>is_\<L>\<^sub>a\<^sub>l\<^sub>l clss \<longleftrightarrow> is_\<L>\<^sub>a\<^sub>l\<^sub>l init\<close>
-proof -
-
-  have \<open>cdcl\<^sub>W_restart_mset.no_strange_atm (state\<^sub>W_of S)\<close>
-    using invs unfolding twl_struct_invs_def cdcl\<^sub>W_restart_mset.cdcl\<^sub>W_all_struct_inv_def S_def
-    by fast
-  then have
-    \<open>set_mset clss = set_mset init\<close>
-    unfolding clss_def init_def S_def
-    by (cases S\<^sub>0) (auto simp: clauses_def mset_take_mset_drop_mset' cdcl\<^sub>W_restart_mset_state
-        cdcl\<^sub>W_restart_mset.no_strange_atm_def in_all_lits_of_mm_ain_atms_of_iff)
-  then show \<open>is_\<L>\<^sub>a\<^sub>l\<^sub>l clss \<longleftrightarrow> is_\<L>\<^sub>a\<^sub>l\<^sub>l init\<close>
-    unfolding is_\<L>\<^sub>a\<^sub>l\<^sub>l_def by blast
-qed
-
 lemma cdcl_twl_o_literals_are_\<L>\<^sub>i\<^sub>n_invs:
   fixes S :: \<open>nat twl_st_wl\<close>
   assumes \<A>\<^sub>i\<^sub>n: \<open>literals_are_\<L>\<^sub>i\<^sub>n S\<^sub>0\<close> and
@@ -1028,14 +1083,6 @@ proof -
       twl_struct_invs_is_\<L>\<^sub>a\<^sub>l\<^sub>l_clauses_init_clss[of T, OF invs_T] init[symmetric]
     .
 qed
-
-lemma set_mset_set_mset_eq_iff: \<open>set_mset A = set_mset B \<longleftrightarrow> (\<forall>a\<in>#A. a \<in># B) \<and> (\<forall>a\<in>#B. a \<in># A)\<close>
-  by blast
-
-lemma is_\<L>\<^sub>a\<^sub>l\<^sub>l_alt_def: \<open>is_\<L>\<^sub>a\<^sub>l\<^sub>l (all_lits_of_mm A) \<longleftrightarrow> atms_of_mm A = atms_of \<L>\<^sub>a\<^sub>l\<^sub>l\<close>
-  unfolding set_mset_set_mset_eq_iff is_\<L>\<^sub>a\<^sub>l\<^sub>l_def Ball_def in_\<L>\<^sub>a\<^sub>l\<^sub>l_atm_of_in_atms_of_iff
-    in_all_lits_of_mm_ain_atms_of_iff
-  by auto (metis literal.sel(2))+
 
 
 lemma skip_and_resolve_loop_wl_D_spec:
@@ -1129,28 +1176,6 @@ definition (in isasat_input_ops) backtrack_wl_D :: "nat twl_st_wl \<Rightarrow> 
         propagate_unit_bt_wl_D L S
      }
   }\<close>
-
-lemma literals_are_\<L>\<^sub>i\<^sub>n_conflict_literals_are_in_\<L>\<^sub>i\<^sub>n:
-  assumes
-    \<A>\<^sub>i\<^sub>n: \<open>literals_are_\<L>\<^sub>i\<^sub>n S\<close> and
-    confl: \<open>get_conflict_wl S \<noteq> None\<close> and
-    struct: \<open>twl_struct_invs (twl_st_of_wl None S)\<close>
-  shows \<open>literals_are_in_\<L>\<^sub>i\<^sub>n (the (get_conflict_wl S))\<close>
-proof -
-  have alien: \<open>cdcl\<^sub>W_restart_mset.no_strange_atm (state\<^sub>W_of (twl_st_of_wl None S))\<close>
-    using struct unfolding twl_struct_invs_def cdcl\<^sub>W_restart_mset.cdcl\<^sub>W_all_struct_inv_def
-    by fast
-  then have N: \<open>atms_of (the (get_conflict_wl S)) \<subseteq> atms_of_mm (init_clss (state\<^sub>W_of (twl_st_of_wl None S)))\<close>
-    using confl unfolding cdcl\<^sub>W_restart_mset.no_strange_atm_def
-    by (cases S; cases \<open>get_conflict_wl S\<close>)
-       (auto simp: cdcl\<^sub>W_restart_mset_state mset_take_mset_drop_mset')
-
-  have \<open>is_\<L>\<^sub>a\<^sub>l\<^sub>l (all_lits_of_mm (init_clss (state\<^sub>W_of (twl_st_of_wl None S))))\<close>
-    using twl_struct_invs_is_\<L>\<^sub>a\<^sub>l\<^sub>l_clauses_init_clss[OF struct] \<A>\<^sub>i\<^sub>n by fast
-  then show ?thesis
-    using N in_all_lits_of_m_ain_atms_of_iff in_all_lits_of_mm_ain_atms_of_iff
-    by (fastforce simp: literals_are_in_\<L>\<^sub>i\<^sub>n_def is_\<L>\<^sub>a\<^sub>l\<^sub>l_def )
-qed
 
 lemma backtrack_wl_D_spec:
   assumes \<A>\<^sub>i\<^sub>n: \<open>literals_are_\<L>\<^sub>i\<^sub>n S\<close> and confl: \<open>get_conflict_wl S ~= None\<close>
